vale/code/arch/x64/interop/Fast_stdcalls.fsti
@@ -1,0 +1,32 @@
+module Fast_stdcalls
+
+open X64.CPU_Features_s
+open FStar.HyperStack.ST
+module B = LowStar.Buffer
+module HS = FStar.HyperStack
+open Fast_defs
+
+unfold
+let u256 = b:B.buffer UInt64.t{B.length b == 4}
+
+let as_nat (b:B.buffer UInt64.t{B.length b == 4}) (h:HS.mem) : GTot nat =
+  let s = B.as_seq h b in
+  let s0 = UInt64.v (Seq.index s 0) in
+  let s1 = UInt64.v (Seq.index s 1) in
+  let s2 = UInt64.v (Seq.index s 2) in
+  let s3 = UInt64.v (Seq.index s 3) in
+  pow2_four s0 s1 s2 s3
+
+val add1
+  (out:u256)
+  (f1:u256)
+  (f2:UInt64.t)
+  : Stack UInt64.t
+  (requires fun h ->
+    adx_enabled /\ bmi2_enabled /\
+    B.live h out /\ B.live h f1 /\
+    B.disjoint out f1)
+  (ensures fun h0 c h1 ->
+    B.live h1 out /\ B.live h1 f1 /\
+    B.modifies (B.loc_buffer out) h0 h1 /\
+    as_nat out h1 + pow2_256 `op_Multiply` UInt64.v c == as_nat f1 h0 + UInt64.v f2)  
